Non-live regions can be removed from modifies

ulib/FStar.HyperStackNG.fst
@@ -276,17 +276,81 @@ let modifies_reference_elim
 
 (* Prove that regions that were not live before and are not live after can be ignored by modifies. *)
 
+abstract
+let rec live_not_live_region_loc_disjoint
+  (r: HH.rid)
+  (h: mem)
+  (#t: Type u#1)
+  (#l: nat)
+  (c: Modifies.class root_class l t)
+  (o: t)
+  (lo: Modifies.loc root_class { TSet.mem lo (locset_of_region_with_liveness r) } )
+: Lemma
+  (requires (Modifies.Class?.live c h o /\ (~ (live_region h r))))
+  (ensures (Modifies.loc_disjoint (Modifies.loc_of_object c o) lo))
+  (decreases l)
+= if l = 0
+  then
+    let _ = Modifies.level_0_class_eq_root c in
+    let c: Modifies.class root_class 0 object = c in
+    let o: object = o in
+    let rg = match o with
+    | ObjectReference _ rf -> frameOf rf
+    | ObjectRegionLiveness rg -> rg
+    in
+    let _ = assert (Modifies.locset_disjoint (locset_of_region_with_liveness rg) (locset_of_region_with_liveness r)) in // TODO: WHY needed?
+    let _ : squash (TSet.mem (Modifies.loc_of_object c o) (locset_of_region_with_liveness rg)) = match o with
+    | ObjectReference _ rf ->
+      locset_of_reference_subset_locset_of_region rg rf // TODO: WHY not triggered?
+    | _ -> ()
+    in
+    ()
+  else
+    let k
+      (i: nat { i < Modifies.Class?.ancestor_count c o } )
+    : Lemma
+      (Modifies.loc_disjoint (Modifies.loc_of_object (Modifies.Class?.ancestor_classes c o i) (Modifies.Class?.ancestor_objects c o i)) lo)
+    = Modifies.live_ancestors c h o i;
+      live_not_live_region_loc_disjoint r h (Modifies.Class?.ancestor_classes c o i) (Modifies.Class?.ancestor_objects c o i) lo
+    in
+    Modifies.loc_disjoint_ancestors_left c o lo k
 
-#reset-options "--z3rlimit 32"
-
+abstract
 let modifies_not_live_region
   (r: HH.rid)
   (s: Modifies.locset root_class)
   (h h': mem)
 : Lemma
-  (requires (Modifies.modifies u#0 u#1 (TSet.union s (locset_of_region_with_liveness r)) h h' /\ (~ (live_region h r)) /\ (~ (live_region h' r))))
+  (requires (Modifies.modifies u#0 u#1 (TSet.union s (locset_of_region_with_liveness r)) h h' /\ (~ (live_region h r))))
   (ensures (Modifies.modifies s h h'))
 = let z : squash (Modifies.modifies u#0 u#1 (TSet.union s (locset_of_region_with_liveness r)) h h') = () in
+  let f'
+    (ty: Type u#1)
+    (l: nat)
+    (c: Modifies.class root_class l ty )
+    (o: ty)
+    (g: (
+      (o' : Modifies.loc root_class { TSet.mem o' s } ) ->
+      Lemma
+      (Modifies.loc_disjoint (Modifies.loc_of_object c o) o')
+    ))
+    ()
+  : Lemma
+    (requires (Modifies.Class?.live c h o))
+    (ensures (Modifies.Class?.preserved c o h h'))
+  = let g'
+      (o': Modifies.loc root_class { TSet.mem o' (TSet.union s (locset_of_region_with_liveness r)) } )
+    : Lemma
+      (Modifies.loc_disjoint (Modifies.loc_of_object c o) o')
+    = Classical.or_elim
+        #(TSet.mem o' s)
+        #(TSet.mem o' (locset_of_region_with_liveness r))
+        #(fun _ -> Modifies.loc_disjoint (Modifies.loc_of_object c o) o')
+        (fun _ -> g o')
+        (fun _ -> live_not_live_region_loc_disjoint r h c o o')
+    in
+    Modifies.modifies_elim (TSet.union s (locset_of_region_with_liveness r)) h h' () c o g'
+  in
   let f
     (ty: Type u#1)
     (l: nat)
@@ -300,75 +364,8 @@ let modifies_not_live_region
   : Lemma
     (requires True)
     (ensures (Modifies.Class?.preserved c o h h'))
-    (decreases l)
-  = if l = 0
-    then begin
-      Modifies.level_0_class_eq_root c;
-      let c: Modifies.class root_class 0 object = c in
-      let o: object = o in
-      match o with
-      | ObjectReference _ rf ->
-        let k
-          ()
-        : Lemma
-          (requires (contains h rf))
-          (ensures (contains h' rf /\ sel h' rf == sel h rf))
-        = let rg = frameOf rf in
-          assert (Modifies.locset_disjoint (locset_of_region_with_liveness rg) (locset_of_region_with_liveness r)); // TODO: WHY needed?
-          locset_of_reference_subset_locset_of_region rg rf; // TODO: WHY not triggered?
-          let g'
-            (o': Modifies.loc root_class { TSet.mem o' (TSet.union s (locset_of_region_with_liveness r)) } )
-          : Lemma
-            (Modifies.loc_disjoint (Modifies.loc_of_object c o) o')
-          = Classical.or_elim
-              #(TSet.mem o' s)
-              #(TSet.mem o' (locset_of_region_with_liveness r))
-              #(fun _ -> Modifies.loc_disjoint (Modifies.loc_of_object c o) o')
-              (fun _ -> g o')
-              (fun _ -> ())
-          in
-          Modifies.modifies_elim (TSet.union s (locset_of_region_with_liveness r)) h h' () c o g'
-        in
-        let v : squash (Modifies.Class?.preserved c o h h') =
-          Classical.move_requires k ()
-        in
-        v
-      | ObjectRegionLiveness rg ->
-        let k
-          ()
-        : Lemma
-          (requires (live_region h rg))
-          (ensures (live_region h' rg))
-        = assert (Modifies.locset_disjoint (locset_of_region_with_liveness rg) (locset_of_region_with_liveness r)); // TODO: WHY WHY WHY is this assert needed?
-          let g'
-            (o': Modifies.loc root_class { TSet.mem o' (TSet.union s (locset_of_region_with_liveness r)) } )
-          : Lemma
-            (Modifies.loc_disjoint (Modifies.loc_of_object c o) o')
-          = Classical.or_elim
-              #(TSet.mem o' s)
-              #(TSet.mem o' (locset_of_region_with_liveness r))
-              #(fun _ -> Modifies.loc_disjoint (Modifies.loc_of_object c o) o')
-              (fun _ -> g o')
-              (fun _ -> ())
-          in
-          Modifies.modifies_elim (TSet.union s (locset_of_region_with_liveness r)) h h' z c o g'
-        in
-        let v : squash (Modifies.Class?.preserved c o h h') =
-          Classical.move_requires k ()
-        in
-        v
-    end else begin
-    (*
-      let g'
-        (i: nat { i < Modifies.Class?.ancestor_count c o } )
-        (o' : Modifies.loc root_class { TSet.mem o' s } )
-      : Lemma
-        (Modifies.loc_disjoint (Modifies.loc_of_object (Modifies.Class?.ancestor_classes c o i) (Modifies.Class?.ancestor_objects c o i)) o')
-      =        
-      in
-      *)
-      assume (Modifies.Class?.preserved c o h h')
-    end
+  = Classical.move_requires (f' ty l c o g) ();
+    Modifies.live_preserved_preserved c h h' o
   in
   Modifies.modifies_intro s h h' f
 
